

# COMP 4190 Assignment 1 Answer

Fidelio Ciandy, 7934456

## Problem 1

For my first question, I have two functions with different purposes.

- **TransformWord**

- This function performs the BFS.
- Starting from the begin word, it performs BFS by comparing the current word with the words in the word list.
- If the current word differs by a single letter, the new word is inserted into the queue and the sequence counter is incremented by 1.
- The visited word is added to a set to prevent circular loops.
- The loop continues until the end word is reached or the queue is empty.

- **CheckAdjacentWords**

- This function will compare two strings and check whether those two strings differ by 1 letter or not

## Problem 2

## Problem 3

## Problem 4

## Problem 5

- (a) The state  $dp[i][j]$  represents the minimum number of edit operations to transform  $s$  into  $t$ . For each value in  $i$  and  $j$ , the table will save the previous minimum comparison between prefixes of  $s[1..i]$  and  $t[1..j]$ , and  $dp[m][n]$  will get the minimum value of the edit operations between the two strings.

For recurrence, where  $i \geq 1, j \geq 1$ :

- $dp[i-1][j] + 1 \rightarrow$  this specify the delete operation, where last character of  $s_i$  is deleted from  $s[1..i]$ , to transform  $s[1..i-1]$  into  $t[1..j]$
- $dp[i][j-1] + 1 \rightarrow$  this specify the insert operation, where we would like to insert character  $t_j$  into string  $s$ , transforming  $s[1..i]$  into  $t[1..j-1]$ .
- $dp[i-1][j-1] + l \rightarrow$  this specify the substitution operation,
  - where if  $s_i = t_j$  we won't add 1, so cost is 0

– otherwise, if  $s_i \neq t_j$ , we will add 1 to substitute the value

(b) The time complexity is  $O(m \times n)$ .

Since the two strings  $s$  and  $t$  have lengths  $m$  and  $n$ ,  $i$  ranges from 0 to  $m$ , and  $j$  ranges from 0 to  $n$  the dp table has  $(m + 1)(n + 1)$  cells.

Futhermore, the calculation of each dp entry using the three recurrences (insertion, deletion, substitution), all of those operations are just accessing the array, thus this can be considered to be  $O(1)$  as the time complexity.

Thus, since each entry is filled using constant number of operations  $O(1)$  and each result is being stored in an  $(m + 1)(n + 1)$  array. Therefore, the time complexity is  $O(m \times n)$ .

(c) The memory/ space complexity of this DP implementation is  $O(m \times n)$ .

Same reasoning as the previous part, since the two strings  $s$  and  $t$  have lengths  $m$  and  $n$ ,  $i$  ranges from 0 to  $m$ , and  $j$  ranges from 0 to  $n$  the dp table has  $(m + 1)(n + 1)$  cells. Thus, the memory complexity is  $O(m \times n)$ .

(d) From the recurrence formula, to fill a row in the DP array, we require only one row from the previous calculation. For instance for  $i=5$ , we only need to access

- $dp[4][5] \rightarrow$  previous row, current column
- $dp[5][4] \rightarrow$  current row, previous column
- $dp[4][4] \rightarrow$  previous row, previous column

Knowing how these calculation work, we could just create two separate array `prev[]` and `curr[]`. Where `prev[]` stores the values of row-1 and `curr[]` stores the current row  $i$ . Thus, this approach reduces the space complexity to  $O(n)$ .

## Problem 6

(a)  $\nabla_x f(x) = \frac{1}{2}(A + A^T)x - b$

Since  $A$  is symmetric, thus,  $A = A^T$

$$\nabla_x f(x) = Ax - b$$

(b)  $x^* : \nabla f(x^*) = 0$

$$Ax^* - b = 0$$

$$Ax^* = b$$

$$A^{-1}(Ax^*) = A^{-1}b$$

$$Ix^* = A^{-1}b$$

$$x^* = A^{-1}b$$

(c)

## Problem 7

(a)  $\nabla f(x) = 2(x - 2)$

(b)  $x_{k+1} = x_k - \alpha \nabla f(x_k)$

$$x_{k+1} = x_k - \alpha 2(x - 2)$$

$$(c) \ x^* : \nabla f(x^*) = 0$$

$$\text{So, } x^* = 2$$

(d) if step size  $\alpha$  is too large: oscillations (no convergence)

if step size  $\alpha$  is too small: slow convergence

$$(e) \ x_{k+1} = x_k - \alpha 2(x - 2)$$

$$= x_k - 2\alpha x_k + 4\alpha$$

$$= (1 - 2\alpha)x_k + 4\alpha$$

Example, let  $(1 - 2\alpha) = b$

$$x_1 = x_0 b + 4\alpha$$

$$x_2 = x_1 b + 4\alpha$$

$$= (x_0 b + 4\alpha)b + 4\alpha$$

$$= x_0 b^2 + 4\alpha b + 4\alpha$$

$$= x_0 b^2 + 4\alpha(b + 1)$$

$$x_3 = x_2 b + 4\alpha$$

$$= (x_0 b^2 + 4\alpha(b + 1))b + 4\alpha$$

$$= (x_0 b^2 + 4\alpha b + 4\alpha)b + 4\alpha$$

$$= x_0 b^3 + 4\alpha b^2 + 4\alpha b + 4\alpha$$

$$= x_0 b^3 + 4\alpha(b^2 + b + 1)$$

So, in general for  $x_k$

$$x_k = x_0 b^k + 4\alpha(b^k + b^{k-1} + \dots + 1)$$

$(b^k + b^{k-1} + \dots + 1)$  is a geometric sum

Thus,

$$x_k = x_0 b^k + 4\alpha \left( \frac{1 - b^k}{1 - b} \right)$$

$$= x_0 b^k + 4\alpha \left( \frac{1 - b^k}{2\alpha} \right)$$

$$= x_0 b^k + 2(1 - b^k)$$

$$= x_0 b^k + 2 - 2b^k$$

$$= (x_0 - 2)b^k + 2$$

$$= (1 - 2\alpha)^k (x_0 - 2) + 2 \quad \dots \text{ sub in } b = (1 - 2\alpha)$$

$x_k$  converges to  $x^* \implies x_k$  converges to 2, since  $x^* = 2$

Thus,  $x_k - 2$  converges to 0

In other word,  $(1 - 2\alpha)^k (x_0 - 2) \rightarrow 0$

Furthermore,  $x_0 \neq x^* \rightarrow x_0 - 2 \neq 0$

Therefore,  $(1 - 2\alpha)^k \rightarrow 0$